sealing/classes.v
@@ -5,18 +5,6 @@ Section WithClasses.
 
 Context {t : machine_types}.
 
-Class sealing_key := {
-  key       : Type
-}.
-
-Context {sk : sealing_key}.
-
-Class sealing_key_ops := {
-  max_key : key;
-  inc_key : key -> key;
-  eq_key :> EqDec (eq_setoid key)
-}.
-
 Class sealing_syscall_addrs := {
   mkkey_addr  : word t;
   seal_addr   : word t;
